\documentclass{article}
\usepackage{amsfonts}
\usepackage{amsmath}
\usepackage{amsthm}
\setlength{\parindent}{0in}\begin{document}
\subsection*{Ex 3 a)}
\begin{equation}
dPS_2  = \frac{d^3k_1}{(2\pi)^32E_1}\frac{d^3k_2}{(2\pi)^32E_2} (2 \pi)^4 \delta^{(4)} (k_1 + k_2 -p_a - p _b)
\end{equation}
\begin{equation}
dPS_2  = \frac{d^3k_1}{(2\pi)^32E_1}\frac{1}{(2\pi)^3} d^4k_2 \delta(k_2^2-m_2^2) (2 \pi)^4 \delta^{(4)} (k_1 + k_2 -p_a - p _b)
\end{equation}
\begin{equation}
dPS_2  = \frac{d^3k_1}{(2\pi)^32E_1}\frac{1}{(2\pi)^3} \delta((p_a+p_b - k_1)^2-m_2^2) (2 \pi)^4
\end{equation}
\begin{equation}
dPS_2  = \frac{d|\vec k_1|d \cos \theta d \phi}{(2\pi)^32E_1}\frac{1}{(2\pi)^3} \delta((p_a+p_b - k_1)^2-m_2^2) (2 \pi)^4 |\vec k_1|
\end{equation}
\begin{equation}
 dE_1 \delta((p_a+p_b - k_1)^2-m_2^2) \overset{\vec p_a = -\vec p_b; p_a^0+p_b^0 = \sqrt{s}}{=}  dE_1 \delta((\sqrt{s} - E_1)^2-m_2^2 - |\vec k_1|^2) = \frac{1}{2|\sqrt{s}|}
\end{equation}
\begin{equation}
 |\vec k_1| = \sqrt{\lambda(s,m_1^2,m_2^2)}/2\sqrt{s} \implies \qed
\end{equation}
\subsection*{Ex 3 b)}
\begin{equation}
dPS_2 = \frac{1}{16\pi^2 2 s}  \sqrt{\lambda(s,m_1^2,m_2^2)} d \cos \theta d \phi 
\end{equation}
\begin{equation}
t = (p_a-k_1)^2 = m_a^2 -2 p_ak_1 + m_1^2 = m_a^2 -2 p_ak_1 + m_1^2 = m_a^2 + m_1^2 - 2(E_aE_1 - \vec p_a\vec p_1 ) =
\end{equation}
\begin{equation}
=t = m_a^2 + m_1^2 - 2(\frac{2+m_a^2-m_b^2}{2\sqrt s} \frac{2+m_1^2-m_2^2}{2\sqrt s} - \frac{ \sqrt{\lambda(s,m_a^2,m_b^2)\lambda(s,m_1^2,m_2^2)} }{4s} \cos \theta)=
\end{equation}
\begin{equation}
t_\pm = t(\theta = 0 \text{ or } \theta=\pi) 
\end{equation}
\begin{equation}
\frac{dt}{d \cos \theta} = \frac{ \sqrt{\lambda(s,m_a^2,m_b^2)\lambda(s,m_1^2,m_2^2)} }{2s} \implies \qed
\end{equation}


\end{document}